coq/LC/Debruijn/F.v
@@ -81,32 +81,29 @@ Fixpoint subst_term n n' ts t :=
   end.
 
 Inductive typing : context typ -> term -> typ -> Prop :=
-  | typvar  : forall ctx n ty, ctxindex ctx n ty -> typing ctx (var n) ty
-  | typapp  : forall ctx t1 t2 ty1 ty2,
-              typing ctx t1 (tyfun ty1 ty2) -> typing ctx t2 ty1 ->
-              typing ctx (app t1 t2) ty2
-  | typabs  : forall ctx t ty1 ty2,
-              typing (some ty1 :: ctx) t ty2 ->
-              typing ctx (abs ty1 t) (tyfun ty1 ty2)
-  | typuapp : forall ctx t ty1 ty2,
-              typing ctx t (tyabs ty1) ->
-              typing ctx (uapp t ty2) (subst_typ 0 [:: ty2] ty1)
-  | typuabs : forall ctx t ty,
-              typing (map (omap (shift_typ 1 0)) ctx) t ty ->
-              typing ctx (uabs t) (tyabs ty).
+  | typvar ctx n ty :
+    ctxindex ctx n ty -> typing ctx (var n) ty
+  | typapp ctx t1 t2 ty1 ty2 :
+    typing ctx t1 (tyfun ty1 ty2) -> typing ctx t2 ty1 ->
+    typing ctx (app t1 t2) ty2
+  | typabs ctx t ty1 ty2 :
+    typing (some ty1 :: ctx) t ty2 -> typing ctx (abs ty1 t) (tyfun ty1 ty2)
+  | typuapp ctx t ty1 ty2 :
+    typing ctx t (tyabs ty1) ->
+    typing ctx (uapp t ty2) (subst_typ 0 [:: ty2] ty1)
+  | typuabs ctx t ty :
+    typing (ctxmap (shift_typ 1 0) ctx) t ty -> typing ctx (uabs t) (tyabs ty).
 
 Reserved Notation "t ->r1 t'" (at level 70, no associativity).
 
 Inductive reduction1 : relation term :=
-  | red1fst  : forall ty t1 t2,
-               app (abs ty t1) t2 ->r1 subst_term 0 0 [:: t2] t1
-  | red1snd  : forall t ty,
-               uapp (uabs t) ty ->r1 typemap (subst_typ^~ [:: ty]) 0 t
-  | red1appl : forall t1 t1' t2, t1 ->r1 t1' -> app t1 t2 ->r1 app t1' t2
-  | red1appr : forall t1 t2 t2', t2 ->r1 t2' -> app t1 t2 ->r1 app t1 t2'
-  | red1abs  : forall ty t t', t ->r1 t' -> abs ty t ->r1 abs ty t'
-  | red1uapp : forall t t' ty, t ->r1 t' -> uapp t ty ->r1 uapp t' ty
-  | red1uabs : forall t t', t ->r1 t' -> uabs t ->r1 uabs t'
+  | red1fst ty t1 t2   : app (abs ty t1) t2 ->r1 subst_term 0 0 [:: t2] t1
+  | red1snd t ty       : uapp (uabs t) ty ->r1 typemap (subst_typ^~ [:: ty]) 0 t
+  | red1appl t1 t1' t2 : t1 ->r1 t1' -> app t1 t2 ->r1 app t1' t2
+  | red1appr t1 t2 t2' : t2 ->r1 t2' -> app t1 t2 ->r1 app t1 t2'
+  | red1abs ty t t'    : t ->r1 t' -> abs ty t ->r1 abs ty t'
+  | red1uapp t t' ty   : t ->r1 t' -> uapp t ty ->r1 uapp t' ty
+  | red1uabs t t'      : t ->r1 t' -> uabs t ->r1 uabs t'
   where "t ->r1 t'" := (reduction1 t t').
 
 Notation reduction := [* reduction1].
@@ -115,67 +112,63 @@ Infix "->r" := reduction (at level 70, no associativity).
 Hint Resolve typvar typapp typabs typuapp typuabs
   red1fst red1snd red1appl red1appr red1abs red1uapp red1uabs.
 
-Lemma shift_zero_ty : forall n t, shift_typ 0 n t = t.
+Lemma shift_zero_ty n t : shift_typ 0 n t = t.
 Proof.
-  move => n t; elim: t n => /=; try congruence.
-  by move => m n; rewrite addn0 if_same.
+  by elim: t n => /=; try congruence; move => m n; rewrite addn0 if_same.
 Qed.
 
-Lemma shift_add_ty :
-  forall d c d' c' t, c <= c' <= d + c ->
+Lemma shift_add_ty d c d' c' t :
+  c <= c' <= d + c ->
   shift_typ d' c' (shift_typ d c t) = shift_typ (d' + d) c t.
 Proof.
-  move => d c d' c' t; case/andP; elimleq; rewrite leq_add2r; elimleq.
-  elim: t c c' => /=; try (move: addnS; congruence); move => *; elimif_omega.
+  case/andP; elimleq; rewrite leq_add2r; elimleq;
+    elim: t c c' => /=; try (move: addnS; congruence); move => *; elimif_omega.
 Qed.
 
-Lemma shift_shift_distr_ty :
-  forall d c d' c' t,
-  c' <= c -> shift_typ d' c' (shift_typ d c t) =
-  shift_typ d (d' + c) (shift_typ d' c' t).
+Lemma shift_shift_distr_ty d c d' c' t :
+  c' <= c ->
+  shift_typ d' c' (shift_typ d c t) = shift_typ d (d' + c) (shift_typ d' c' t).
 Proof.
-  move => d c d' c' t; elimleq; elim: t c c' => /=;
+  elimleq; elim: t c c' => /=;
     try (move: addnS; congruence); move => *; elimif_omega.
 Qed.
 
-Lemma shift_subst_distr_ty :
-  forall n d c ts t, c <= n ->
+Lemma shift_subst_distr_ty n d c ts t :
+  c <= n ->
   shift_typ d c (subst_typ n ts t) = subst_typ (d + n) ts (shift_typ d c t).
 Proof.
-  move => n d c ts t; elimleq; elim: t n c => /=;
+  elimleq; elim: t n c => /=;
     try (move: addnS; congruence); move => v n c; elimif_omega.
   by rewrite /subst_typv shift_add_ty ?addn0 ?leq_addl // !subnDA addnK.
 Qed.
 
-Lemma subst_shift_distr_ty :
-  forall n d c ts t,
+Lemma subst_shift_distr_ty n d c ts t :
   shift_typ d (n + c) (subst_typ n ts t) =
   subst_typ n (map (shift_typ d c) ts) (shift_typ d (size ts + n + c) t).
 Proof.
-  move => n d c ts t; elim: t n => /=; try (move: addnS addSn; congruence).
-  move => m n; rewrite /subst_typv size_map; elimif_omega.
+  elim: t n => /=; try (move: addnS addSn; congruence);
+    move => m n; rewrite /subst_typv size_map; elimif_omega.
   - rewrite !nth_default ?size_map /=; try ssromega.
     rewrite (subnAC _ n) subnK; elimif_omega.
   - rewrite -shift_shift_distr_ty // nth_map' /=.
     f_equal; apply nth_equal; rewrite size_map; elimif_omega.
 Qed.
 
-Lemma subst_shift_cancel_ty :
-  forall n d c ts t, c <= n -> size ts + n <= d + c ->
+Lemma subst_shift_cancel_ty n d c ts t :
+  c <= n -> size ts + n <= d + c ->
   subst_typ n ts (shift_typ d c t) = shift_typ (d - size ts) c t.
 Proof.
-  move => n d c ts t; elimleq; rewrite addnA leq_add2r; elimleq.
+  elimleq; rewrite addnA leq_add2r; elimleq.
   elim: t n c => /=; try (move: addnS; congruence); move => v n c;
     elimif_omega; rewrite /subst_typv nth_default /=; f_equal; ssromega.
 Qed.
 
-Lemma subst_subst_distr_ty :
-  forall n m xs ys t,
+Lemma subst_subst_distr_ty n m xs ys t :
   subst_typ (m + n) xs (subst_typ m ys t) =
   subst_typ m (map (subst_typ n xs) ys) (subst_typ (size ys + m + n) xs t).
 Proof.
-  move => n m xs ys t; elim: t m => /=; try (move: addnS addSn; congruence).
-  move => v m; elimif_omega; rewrite /subst_typv.
+  elim: t m => /=; try (move: addnS addSn; congruence);
+    move => v m; elimif_omega; rewrite /subst_typv.
   - rewrite (subst_shift_cancel_ty m) // size_map
       ?addn0 ?leq_addr // -{1}addnA addKn nth_default /=; last ssromega.
     rewrite /subst_typv subnAC subnK ?subnDA; elimif_omega.
@@ -183,29 +176,27 @@ Proof.
     apply nth_equal; rewrite size_map /=; elimif_omega.
 Qed.
 
-Lemma subst_app_ty :
-  forall n xs ys t,
+Lemma subst_app_ty n xs ys t :
   subst_typ n xs (subst_typ (size xs + n) ys t) = subst_typ n (xs ++ ys) t.
 Proof.
-  move => n xs ys t; elim: t n => /=; try (move: addnS; congruence).
-  move => v n; elimif_omega; rewrite /subst_typv.
+  elim: t n => /=; try (move: addnS; congruence);
+    move => v n; elimif_omega; rewrite /subst_typv.
   - rewrite subst_shift_cancel_ty ?addn0 //
       size_cat nth_cat !subnDA addKn (subnAC _ (size xs)); elimif_omega.
   - rewrite nth_cat; f_equal; elimif_omega; apply nth_equal; ssromega.
 Qed.
 
-Lemma subst_nil_ty : forall n t, subst_typ n [::] t = t.
+Lemma subst_nil_ty n t : subst_typ n [::] t = t.
 Proof.
-  move => n t; elim: t n => /=; try congruence.
-  move => v n; rewrite /subst_typv nth_nil /= -fun_if; elimif_omega.
+  elim: t n => /=; try congruence;
+    move => v n; rewrite /subst_typv nth_nil /= -fun_if; elimif_omega.
 Qed.
 
-Lemma typemap_compose :
-  forall f g n m t,
+Lemma typemap_compose f g n m t :
   typemap f n (typemap g m t) =
   typemap (fun i ty => f (i + n) (g (i + m) ty)) 0 t.
 Proof.
-  move => f g n m t; elim: t n m => //=.
+  elim: t n m => //=.
   - by move => tl IHtl tr IHtr n m; rewrite IHtl IHtr.
   - by move => ty t IH n m; rewrite IH.
   - by move => t IH ty n m; rewrite IH.
@@ -213,200 +204,183 @@ Proof.
     elim: t (0) => //=; move: addSnnS; congruence.
 Qed.
 
-Lemma typemap_eq' :
-  forall f g n m t,
+Lemma typemap_eq' f g n m t :
   (forall o t, f (o + n) t = g (o + m) t) -> typemap f n t = typemap g m t.
 Proof.
-  move => f g n m t H; elim: t n m H => //=.
+  move => H; elim: t n m H => //=.
   - by move => tl IHtl tr IHtr n m H; f_equal; auto.
   - by move => ty t IH n m H; f_equal; auto; rewrite -(add0n n) -(add0n m).
   - by move => t IH ty n m H; f_equal; auto; rewrite -(add0n n) -(add0n m).
   - by move => t IH n m H; f_equal; apply IH => o ty; rewrite -!addSnnS.
 Qed.
 
-Lemma typemap_eq :
-  forall f g n t, (forall n t, f n t = g n t) -> typemap f n t = typemap g n t.
+Lemma typemap_eq f g n t :
+  (forall n t, f n t = g n t) -> typemap f n t = typemap g n t.
 Proof.
-  move => f g n t H; apply typemap_eq' => {t} o; apply H.
+  move => H; apply typemap_eq' => {t} o; apply H.
 Qed.
 
-Lemma shifttyp_zero : forall c t, typemap (shift_typ 0) c t = t.
+Lemma shifttyp_zero c t : typemap (shift_typ 0) c t = t.
 Proof.
-  move => c t; elim: t c => /=; move: shift_zero_ty; congruence.
+  elim: t c => /=; move: shift_zero_ty; congruence.
 Qed.
 
-Lemma shifttyp_add :
-  forall d c d' c' t, c <= c' <= d + c ->
+Lemma shifttyp_add d c d' c' t :
+  c <= c' <= d + c ->
   typemap (shift_typ d') c' (typemap (shift_typ d) c t) =
   typemap (shift_typ (d' + d)) c t.
 Proof.
-  move => d c d' c' t H.
-  rewrite typemap_compose. apply typemap_eq' => {t} n t.
+  rewrite typemap_compose => H; apply typemap_eq' => {t} n t.
   by rewrite addn0 shift_add_ty // addnCA !leq_add2l.
 Qed.
 
-Lemma shifttyp_shifttyp_distr :
-  forall d c d' c' t, c' <= c ->
+Lemma shifttyp_shifttyp_distr d c d' c' t :
+  c' <= c ->
   typemap (shift_typ d') c' (typemap (shift_typ d) c t) =
   typemap (shift_typ d) (d' + c) (typemap (shift_typ d') c' t).
 Proof.
-  move => d c d' c' t H.
-  rewrite !typemap_compose; apply typemap_eq => {t} n t.
+  rewrite !typemap_compose => H; apply typemap_eq => {t} n t.
   by rewrite shift_shift_distr_ty ?leq_add2l // addnCA.
 Qed.
 
-Lemma shifttyp_substtyp_distr :
-  forall n d c ts t, c <= n ->
+Lemma shifttyp_substtyp_distr n d c ts t :
+  c <= n ->
   typemap (shift_typ d) c (typemap (subst_typ^~ ts) n t) =
   typemap (subst_typ^~ ts) (d + n) (typemap (shift_typ d) c t).
 Proof.
-  move => n d c ts t H.
-  rewrite !typemap_compose; apply typemap_eq => {t} n' t.
+  rewrite !typemap_compose => H; apply typemap_eq => {t} n' t.
   by rewrite shift_subst_distr_ty ?leq_add2l // addnCA.
 Qed.
 
-Lemma substtyp_shifttyp_distr :
-  forall n d c ts t,
+Lemma substtyp_shifttyp_distr n d c ts t :
   typemap (shift_typ d) (n + c) (typemap (subst_typ^~ ts) n t) =
   typemap (subst_typ^~ (map (shift_typ d c) ts)) n
     (typemap (shift_typ d) (size ts + n + c) t).
 Proof.
-  move => n d c ts t.
   rewrite !typemap_compose; apply typemap_eq => {t} n' t.
   by rewrite addnA subst_shift_distr_ty !addnA (addnC (size _)).
 Qed.
 
-Lemma substtyp_substtyp_distr :
-  forall n m xs ys t,
+Lemma substtyp_substtyp_distr n m xs ys t :
   typemap (subst_typ^~ xs) (m + n) (typemap (subst_typ^~ ys) m t) =
   typemap (subst_typ^~ (map (subst_typ n xs) ys)) m
     (typemap (subst_typ^~ xs) (size ys + m + n) t).
 Proof.
-  move => n m xs ys t.
   rewrite !typemap_compose; apply typemap_eq => {t} n' t.
   by rewrite addnA subst_subst_distr_ty !addnA (addnC (size _)).
 Qed.
 
-Lemma shift_typemap_distr :
-  forall f d c n t,
+Lemma shift_typemap_distr f d c n t :
   shift_term d c (typemap f n t) = typemap f n (shift_term d c t).
 Proof.
-  move => f d c n t; elim: t d c n => /=; congruence.
+  elim: t d c n => /=; congruence.
 Qed.
 
-Lemma subst_shifttyp_distr :
-  forall n m d c ts t, c <= m ->
+Lemma subst_shifttyp_distr n m d c ts t :
+  c <= m ->
   subst_term n (d + m) ts (typemap (shift_typ d) c t) =
   typemap (shift_typ d) c (subst_term n m ts t).
 Proof.
-  move => m n d c ts t; elimleq; elim: t n m c => /=;
-    try (move: addnS; congruence); move => v n m c; elimif_omega.
-  by rewrite /subst_termv -!shift_typemap_distr shifttyp_add //
-    addn0 leq_addl.
+  elimleq; elim: t n m c => /=; try (move: addnS; congruence);
+    move => v n m c; elimif_omega.
+  by rewrite /subst_termv -!shift_typemap_distr shifttyp_add // addn0 leq_addl.
 Qed.
 
-Lemma shifttyp_subst_distr :
-  forall d c n m ts t,
+Lemma shifttyp_subst_distr d c n m ts t :
   typemap (shift_typ d) (m + c) (subst_term n m ts t) =
   subst_term n m (map (typemap (shift_typ d) c) ts)
     (typemap (shift_typ d) (m + c) t).
 Proof.
-  move => d c n m ts t; elim: t n m => /=; try (move: addSn; congruence).
-  move => v n m; elimif_omega.
+  elim: t n m => /=; try (move: addSn; congruence); move => v n m; elimif_omega.
   by rewrite /subst_termv size_map -!shift_typemap_distr
     -shifttyp_shifttyp_distr // (nth_map' (typemap _ _)).
 Qed.
 
-Lemma subst_substtyp_distr :
-  forall n m m' tys ts t, m' <= m ->
+Lemma subst_substtyp_distr n m m' tys ts t :
+  m' <= m ->
   subst_term n m ts (typemap (subst_typ^~ tys) m' t) =
   typemap (subst_typ^~ tys) m' (subst_term n (size tys + m) ts t).
 Proof.
-  move => n m m' tys ts t; elimleq; elim: t n m m' => /=;
-    try (move: addnS; congruence); move => v n m m'; elimif_omega.
+  elimleq; elim: t n m m' => /=; try (move: addnS; congruence);
+    move => v n m m'; elimif_omega.
   rewrite /subst_termv -!shift_typemap_distr typemap_compose.
   f_equal; apply typemap_eq => {v n ts H} n t.
   rewrite addn0 subst_shift_cancel_ty ?addKn //; ssromega.
 Qed.
 
-Lemma substtyp_subst_distr :
-  forall n m m' tys ts t, m <= m' ->
+Lemma substtyp_subst_distr n m m' tys ts t :
+  m <= m' ->
   typemap (subst_typ^~ tys) m' (subst_term n m ts t) =
   subst_term n m (map (typemap (subst_typ^~ tys) (m' - m)) ts)
     (typemap (subst_typ^~ tys) m' t).
 Proof.
-  move => n m m' tys ts t; elimleq; elim: t n m m' => /=;
-    try (move: addnS; congruence); move => v n m m'; elimif_omega.
+  elimleq; elim: t n m m' => /=; try (move: addnS; congruence);
+    move => v n m m'; elimif_omega.
   by rewrite /subst_termv size_map -!shift_typemap_distr
     addnC -shifttyp_substtyp_distr // (nth_map' (typemap _ _)) /=.
 Qed.
 
-Lemma shift_zero : forall n t, shift_term 0 n t = t.
+Lemma shift_zero n t : shift_term 0 n t = t.
 Proof.
-  move => n t; elim: t n => /=; try congruence.
-  by move => m n; rewrite addn0 if_same.
+  by elim: t n => /=; try congruence; move => m n; rewrite addn0 if_same.
 Qed.
 
-Lemma shift_add :
-  forall d c d' c' t, c <= c' <= d + c ->
+Lemma shift_add d c d' c' t :
+  c <= c' <= d + c ->
   shift_term d' c' (shift_term d c t) = shift_term (d' + d) c t.
 Proof.
-  move => d c d' c' t; case/andP; elimleq; rewrite leq_add2r; elimleq;
+  case/andP; elimleq; rewrite leq_add2r; elimleq;
     elim: t c c' => /=; try (move: addnS; congruence); move => *; elimif_omega.
 Qed.
 
-Lemma shift_shift_distr :
-  forall d c d' c' t, c' <= c ->
+Lemma shift_shift_distr d c d' c' t :
+  c' <= c ->
   shift_term d' c' (shift_term d c t) =
   shift_term d (d' + c) (shift_term d' c' t).
 Proof.
-  move => d c d' c' t; elimleq; elim: t c c' => /=;
-    try (move: addnS; congruence); move => v c c'; elimif_omega.
+  elimleq; elim: t c c' => /=; try (move: addnS; congruence);
+    move => v c c'; elimif_omega.
 Qed.
 
-Lemma subst_shift_distr :
-  forall n m d c ts t,
+Lemma subst_shift_distr n m d c ts t :
   shift_term d (n + c) (subst_term n m ts t) =
   subst_term n m (map (shift_term d c) ts) (shift_term d (size ts + n + c) t).
 Proof.
-  move => n m d c ts t; elim: t n m => /=; try (move: addnS addSn; congruence).
-  move => v n m; rewrite /subst_termv size_map; elimif_omega.
+  elim: t n m => /=; try (move: addnS addSn; congruence);
+    move => v n m; rewrite /subst_termv size_map; elimif_omega.
   - rewrite shift_typemap_distr !nth_default ?size_map /=; try ssromega.
     rewrite (subnAC _ n) subnK; elimif_omega.
   - rewrite shift_typemap_distr -shift_shift_distr // nth_map' /=.
     do 2 f_equal; apply nth_equal; rewrite size_map; elimif_omega.
 Qed.
 
-Lemma shift_subst_distr :
-  forall n m d c ts t, c <= n ->
+Lemma shift_subst_distr n m d c ts t :
+  c <= n ->
   shift_term d c (subst_term n m ts t) =
   subst_term (d + n) m ts (shift_term d c t).
 Proof.
-  move => n m d c ts t; elimleq; elim: t n m c => /=;
-    try (move: addnS; congruence); move => v n m c; elimif_omega.
+  elimleq; elim: t n m c => /=; try (move: addnS; congruence);
+    move => v n m c; elimif_omega.
   by rewrite /subst_termv shift_typemap_distr
     (subnDA d) addnK shift_add // addn0 leq_addl.
 Qed.
 
-Lemma subst_shift_cancel :
-  forall n m d c ts t, c <= n -> size ts + n <= d + c ->
+Lemma subst_shift_cancel n m d c ts t :
+  c <= n -> size ts + n <= d + c ->
   subst_term n m ts (shift_term d c t) = shift_term (d - size ts) c t.
 Proof.
-  move => n m d c ts t; elimleq; rewrite addnA leq_add2r; elimleq;
-    elim: t n m c => /=; try (move: addnS; congruence);
-    move => v n m c; elimif_omega.
+  elimleq; rewrite addnA leq_add2r; elimleq; elim: t n m c => /=;
+    try (move: addnS; congruence); move => v n m c; elimif_omega.
   rewrite /subst_termv nth_default /=; f_equal; ssromega.
 Qed.
 
-Lemma subst_subst_distr :
-  forall n n' m m' xs ys t,
+Lemma subst_subst_distr n n' m m' xs ys t :
   subst_term (n' + n) (m' + m) xs (subst_term n' m' ys t) =
   subst_term n' m' (map (subst_term n m xs) ys)
     (subst_term (size ys + n' + n) (m' + m) xs t).
 Proof.
-  move => n n' m m' xs ys t; elim: t n' m' => /=;
-    try (move: addSn addnS; congruence).
-  move => v n' m'; elimif_omega; rewrite /subst_termv.
+  elim: t n' m' => /=; try (move: addSn addnS; congruence);
+    move => v n' m'; elimif_omega; rewrite /subst_termv.
   - rewrite -!shift_typemap_distr (subst_shift_cancel n') // size_map
       ?addn0 ?leq_addr // nth_default /= /subst_termv; elimif_omega.
     by rewrite shift_typemap_distr -addnA addKn subnDA addnK addnCA !subnDA.
@@ -416,30 +390,28 @@ Proof.
     rewrite size_map; elimif_omega.
 Qed.
 
-Lemma subst_app :
-  forall n m xs ys t,
+Lemma subst_app n m xs ys t :
   subst_term n m xs (subst_term (size xs + n) m ys t) =
   subst_term n m (xs ++ ys) t.
 Proof.
-  move => n m xs ys t; elim: t n m => /=; try (move: addnS; congruence).
+  elim: t n m => /=; try (move: addnS; congruence).
   move => v n m; rewrite /subst_termv nth_cat size_cat; elimif_omega.
   - by rewrite -!shift_typemap_distr subst_shift_cancel
       ?addn0 // addKn addnC !subnDA.
   - rewrite /subst_termv; do 2 f_equal; apply nth_equal; ssromega.
 Qed.
 
-Lemma subst_nil : forall n m t, subst_term n m [::] t = t.
+Lemma subst_nil n m t : subst_term n m [::] t = t.
 Proof.
-  move => n m t; elim: t n m => /=; try congruence.
+  elim: t n m => /=; try congruence.
   move => v n m; rewrite /subst_termv nth_nil /= -fun_if; elimif_omega.
 Qed.
 
-Lemma subst_shifttyp_app :
-  forall n m m' ts t,
+Lemma subst_shifttyp_app n m m' ts t :
   subst_term n m (map (typemap (shift_typ m') 0) ts) t =
   subst_term n (m' + m) ts t.
 Proof.
-  move => n m m' ts t; elim: t n m m' => /=; try (move: addnS; congruence).
+  elim: t n m m' => /=; try (move: addnS; congruence).
   move => v n m m'; rewrite /subst_termv size_map; elimif_omega.
   move: H; elimleq.
   rewrite -!shift_typemap_distr !(nth_map' (typemap _ _)) /=; do 2 f_equal.
@@ -448,44 +420,41 @@ Proof.
   by rewrite addn0 shift_add_ty ?leqnn ?leq_addl // addnC.
 Qed.
 
-Lemma redappl :
-  forall t1 t1' t2, t1 ->r t1' -> app t1 t2 ->r app t1' t2.
+Lemma redappl t1 t1' t2 : t1 ->r t1' -> app t1 t2 ->r app t1' t2.
 Proof.
-  move => t1 t1' t2; elim => // {t1 t1'} t1 t1' t1'' H H0 H1.
+  elim => // {t1 t1'} t1 t1' t1'' H H0 H1.
   by apply rt1n_trans with (app t1' t2) => //; constructor.
 Qed.
 
-Lemma redappr :
-  forall t1 t2 t2', t2 ->r t2' -> app t1 t2 ->r app t1 t2'.
+Lemma redappr t1 t2 t2' : t2 ->r t2' -> app t1 t2 ->r app t1 t2'.
 Proof.
-  move => t1 t2 t2'; elim => // {t2 t2'} t2 t2' t2'' H H0 H1.
+  elim => // {t2 t2'} t2 t2' t2'' H H0 H1.
   by apply rt1n_trans with (app t1 t2') => //; constructor.
 Qed.
 
-Lemma redabs : forall ty t t', t ->r t' -> abs ty t ->r abs ty t'.
+Lemma redabs ty t t' : t ->r t' -> abs ty t ->r abs ty t'.
 Proof.
-  move => ty t t'; elim => // {t t'} t t' t'' H H0 H1.
+  elim => // {t t'} t t' t'' H H0 H1.
   by apply rt1n_trans with (abs ty t') => //; constructor.
 Qed.
 
-Lemma reduapp : forall t t' ty, t ->r t' -> uapp t ty ->r uapp t' ty.
+Lemma reduapp t t' ty : t ->r t' -> uapp t ty ->r uapp t' ty.
 Proof.
-  move => t t' ty; elim => // {t t'} t t' t'' H H0 H1.
+  elim => // {t t'} t t' t'' H H0 H1.
   by apply rt1n_trans with (uapp t' ty) => //; constructor.
 Qed.
 
-Lemma reduabs : forall t t', t ->r t' -> uabs t ->r uabs t'.
+Lemma reduabs t t' : t ->r t' -> uabs t ->r uabs t'.
 Proof.
-  move => t t'; elim => // {t t'} t t' t'' H H0 H1.
+  elim => // {t t'} t t' t'' H H0 H1.
   by apply rt1n_trans with (uabs t') => //; constructor.
 Qed.
 
 Hint Resolve redappl redappr redabs reduapp reduabs.
 
-Lemma typvar_seqindex :
-  forall ctx n ty, typing ctx (var n) ty <-> ctxindex ctx n ty.
+Lemma typvar_seqindex ctx n ty : typing ctx (var n) ty <-> ctxindex ctx n ty.
 Proof.
-  move => ctx n ty; split => H.
+  split => H.
   - by inversion H.
   - by constructor.
 Qed.
@@ -495,16 +464,17 @@ Module confluence_proof.
 Reserved Notation "t ->rp t'" (at level 70, no associativity).
 
 Inductive parred : relation term :=
-  | parredfst  : forall ty t1 t1' t2 t2', t1 ->rp t1' -> t2 ->rp t2' ->
-                 app (abs ty t1) t2 ->rp subst_term 0 0 [:: t2'] t1'
-  | parredsnd  : forall t t' ty, t ->rp t' ->
-                 uapp (uabs t) ty ->rp typemap (subst_typ^~ [:: ty]) 0 t'
-  | parredvar  : forall n, var n ->rp var n
-  | parredapp  : forall t1 t1' t2 t2',
-                 t1 ->rp t1' -> t2 ->rp t2' -> app t1 t2 ->rp app t1' t2'
-  | parredabs  : forall ty t t', t ->rp t' -> abs ty t ->rp abs ty t'
-  | parreduapp : forall t t' ty, t ->rp t' -> uapp t ty ->rp uapp t' ty
-  | parreduabs : forall t t', t ->rp t' -> uabs t ->rp uabs t'
+  | parredfst ty t1 t1' t2 t2' :
+    t1 ->rp t1' -> t2 ->rp t2' ->
+    app (abs ty t1) t2 ->rp subst_term 0 0 [:: t2'] t1'
+  | parredsnd  t t' ty :
+    t ->rp t' -> uapp (uabs t) ty ->rp typemap (subst_typ^~ [:: ty]) 0 t'
+  | parredvar n : var n ->rp var n
+  | parredapp t1 t1' t2 t2' :
+    t1 ->rp t1' -> t2 ->rp t2' -> app t1 t2 ->rp app t1' t2'
+  | parredabs ty t t' : t ->rp t' -> abs ty t ->rp abs ty t'
+  | parreduapp t t' ty : t ->rp t' -> uapp t ty ->rp uapp t' ty
+  | parreduabs t t' : t ->rp t' -> uabs t ->rp uabs t'
   where "t ->rp t'" := (parred t t').
 
 Fixpoint reduce_all_redex t : term :=
@@ -520,9 +490,9 @@ Fixpoint reduce_all_redex t : term :=
     | uabs t => uabs (reduce_all_redex t)
   end.
 
-Lemma parred_refl : forall t, parred t t.
+Lemma parred_refl t : parred t t.
 Proof.
-  by elim; constructor.
+  by elim: t; constructor.
 Qed.
 
 Hint Resolve
@@ -547,21 +517,20 @@ Proof.
   - move => t1 t1' t2 t2' H H0 H1 H2; apply rtc_trans' with (app t1 t2'); auto.
 Qed.
 
-Lemma shift_parred :
-  forall t t' d c, t ->rp t' -> shift_term d c t ->rp shift_term d c t'.
+Lemma shift_parred t t' d c :
+  t ->rp t' -> shift_term d c t ->rp shift_term d c t'.
 Proof.
-  move => t t' d c H; move: t t' H d c.
+  move => H; move: t t' H d c.
   refine (parred_ind _ _ _ _ _ _ _ _) => //=; try by constructor.
   - by move => ty t1 t1' t2 t2' H H0 H1 H2 d c;
       rewrite (subst_shift_distr 0) /= !add1n; auto.
   - by move => t t' ty H H0 d c; rewrite shift_typemap_distr; auto.
 Qed.
 
-Lemma shifttyp_parred :
-  forall t t' d c,
+Lemma shifttyp_parred t t' d c :
   t ->rp t' -> typemap (shift_typ d) c t ->rp typemap (shift_typ d) c t'.
 Proof.
-  move => t t' d c H; move: t t' H d c.
+  move => H; move: t t' H d c.
   refine (parred_ind _ _ _ _ _ _ _ _) => /=; auto.
   - by move => ty t1 t1' t2 t2' H H0 H1 H2 d c;
       rewrite (shifttyp_subst_distr d c 0 0) add0n /=; auto.
@@ -569,11 +538,11 @@ Proof.
       rewrite -{3}(add0n m) substtyp_shifttyp_distr /= 2!add1n; auto.
 Qed.
 
-Lemma substtyp_parred :
-  forall n tys t t', t ->rp t' ->
+Lemma substtyp_parred n tys t t' :
+  t ->rp t' ->
   typemap (subst_typ^~ tys) n t ->rp typemap (subst_typ^~ tys) n t'.
 Proof.
-  move => n tys t t' H; move: t t' H n.
+  move => H; move: t t' H n.
   refine (parred_ind _ _ _ _ _ _ _ _) => /=; auto.
   - by move => ty t1 t1' t2 t2' H H0 H1 H2 n;
       rewrite substtyp_subst_distr //= subn0; auto.
@@ -581,12 +550,12 @@ Proof.
       rewrite -{3}(add0n n) substtyp_substtyp_distr /= 2!add1n; auto.
 Qed.
 
-Lemma subst_parred :
-  forall n m ps t t', Forall (prod_curry parred) ps -> t ->rp t' ->
+Lemma subst_parred n m ps t t' :
+  Forall (prod_curry parred) ps -> t ->rp t' ->
   subst_term n m [seq fst p | p <- ps] t ->rp
   subst_term n m [seq snd p | p <- ps] t'.
 Proof.
-  move => n m ps t t' H H0; move: t t' H0 n m.
+  move => H H0; move: t t' H0 n m.
   refine (parred_ind _ _ _ _ _ _ _ _) => /=; auto.
   - by move => ty tl tl' tr tr' H0 H1 H2 H3 n m;
       rewrite (subst_subst_distr n 0 m 0) /= 2!add1n add0n; auto.
@@ -599,9 +568,9 @@ Proof.
     - by rewrite subSS; apply IH.
 Qed.
 
-Lemma parred_all_lemma : forall t t', t ->rp t' -> t' ->rp reduce_all_redex t.
+Lemma parred_all_lemma t t' : t ->rp t' -> t' ->rp reduce_all_redex t.
 Proof with auto.
-  fix 3 => t t' H; inversion H; subst => {H} /=; try by constructor; auto.
+  move: t t'; fix 3 => t t' H; inversion H; subst => {H} /=; auto.
   - apply (subst_parred 0 0 [:: (t2', reduce_all_redex t2)]) => /=; auto.
   - by apply substtyp_parred; apply parred_all_lemma.
   - by destruct t1; auto; inversion H0; auto.
@@ -624,22 +593,21 @@ End confluence_proof.
 
 Module subject_reduction_proof.
 
-Lemma ctxleq_preserves_typing :
-  forall ctx1 ctx2 t ty, ctx1 <=c ctx2 -> typing ctx1 t ty -> typing ctx2 t ty.
+Lemma ctxleq_preserves_typing ctx1 ctx2 t ty :
+  ctx1 <=c ctx2 -> typing ctx1 t ty -> typing ctx2 t ty.
 Proof.
-  move => ctx1 ctx2 t ty H H0; move: ctx1 t ty H0 ctx2 H.
+  move => H H0; move: ctx1 t ty H0 ctx2 H.
   refine (typing_ind _ _ _ _ _ _); eauto.
   - by move => ctx t ty1 ty2 _ H ctx2 H0; constructor; apply H; case.
   - by move => ctx t ty _ H ctx2 H0; constructor; apply H, ctxleq_map.
 Qed.
 
-Lemma shifttyp_preserves_typing :
-  forall d c ctx t ty,
+Lemma shifttyp_preserves_typing d c ctx t ty :
   typing ctx t ty ->
-  typing (map (omap (shift_typ d c)) ctx)
+  typing (ctxmap (shift_typ d c) ctx)
     (typemap (shift_typ d) c t) (shift_typ d c ty).
 Proof.
-  move => d c ctx t ty H; move: ctx t ty H d c.
+  move => H; move: ctx t ty H d c.
   refine (typing_ind _ _ _ _ _ _) => /=.
   - by move => ctx n ty H d c; apply typvar, ctxindex_map.
   - move => ctx t1 t2 ty1 ty2 _ H _ H0 d c.
@@ -659,13 +627,12 @@ Proof.
       by do 2 f_equal; rewrite (shift_shift_distr_ty d c).
 Qed.
 
-Lemma substtyp_preserves_typing :
-  forall n tys ctx t ty,
+Lemma substtyp_preserves_typing n tys ctx t ty :
   typing ctx t ty ->
-  typing (map (omap (subst_typ n tys)) ctx)
+  typing (ctxmap (subst_typ n tys) ctx)
     (typemap (subst_typ^~ tys) n t) (subst_typ n tys ty).
 Proof.
-  move => n tys ctx t ty H; move: ctx t ty H n.
+  move => H; move: ctx t ty H n.
   refine (typing_ind _ _ _ _ _ _) => /=.
   - move => ctx n ty H v; constructor.
     by rewrite -(nth_map' (omap (subst_typ v tys)) None) -H.
@@ -676,38 +643,31 @@ Proof.
     rewrite -{4}(add0n n) subst_subst_distr_ty /= !add1n.
     by constructor.
   - move => ctx t ty _ H n; constructor.
-    move: {H} (H n.+1); rewrite -!map_comp /funcomp.
-    set ctx1 := map _ _.
-    set ctx2 := map _ _.
-    have -> //: ctx1 = ctx2.
-      rewrite {}/ctx1 {}/ctx2.
-      elim: ctx {t ty} => //= [[ty |]] ctx -> //=.
-      by rewrite shift_subst_distr_ty.
+    move: {H} (H n.+1); apply ssr_congr_arrow; f_equal; first by move ->.
+    elim: ctx {t ty} => //= [[ty |]] ctx -> //=.
+    by rewrite shift_subst_distr_ty.
 Qed.
 
-Lemma subject_shift :
-  forall t ty c ctx1 ctx2,
+Lemma subject_shift t ty c ctx1 ctx2 :
   typing ctx1 t ty ->
   typing (ctxinsert ctx2 ctx1 c) (shift_term (size ctx2) c t) ty.
 Proof.
-  move => t ty c ctx1 ctx2 H; move: ctx1 t ty H c ctx2.
-  refine (typing_ind _ _ _ _ _ _) => /=.
+  move => H; move: ctx1 t ty H c ctx2.
+  refine (typing_ind _ _ _ _ _ _) => /=; auto.
   - move => ctx1 n ty H c ctx2; constructor.
     rewrite {}H nth_ctxinsert; elimif_omega.
   - by move => ctx1 t1 t2 ty1 ty2 _ H _ H0 c ctx2; apply typapp with ty1; auto.
   - by move => ctx1 t ty1 ty2 _ H c ctx2; apply typabs, (H c.+1).
-  - by move => ctx1 t ty1 ty2 _ H c ctx2; constructor; auto.
   - move => ctx1 t ty _ H c ctx2; constructor.
     by rewrite map_ctxinsert -(size_map (omap (shift_typ 1 0)) ctx2).
 Qed.
 
-Lemma subject_subst :
-  forall t ty n ctx ctx',
+Lemma subject_subst t ty n ctx ctx' :
   Forall (fun p => typing (drop n ctx) p.1 p.2) ctx' ->
   typing (ctxinsert [seq Some p.2 | p <- ctx'] ctx n) t ty ->
   typing ctx (subst_term n 0 [seq p.1 | p <- ctx'] t) ty.
 Proof.
-  move => t ty n ctx ctx' H.
+  move => H.
   move: {2 3}(ctxinsert _ _ _)
     (erefl (ctxinsert [seq Some p.2 | p <- ctx'] ctx n)) => ctx'' H0 H1.
   move: ctx'' t ty H1 n ctx ctx' H H0.
@@ -726,8 +686,7 @@ Proof.
           drop_take_nil size_take -!catA /= -{4}(cat_take_drop n ctx).
         apply ctxleq_app => //; case/orP: (leq_total n (size ctx)).
         - by move/minn_idPl => ->; rewrite subnn.
-        - by move => H;
-            rewrite drop_oversize // cats0 => m x; rewrite nth_nseq if_same.
+        - by move => H m x; rewrite (drop_oversize H) cats0 nth_nseq if_same.
       - by rewrite subSS; apply IH.
     - move: H H1 {H2}; elimleq; move/negbT;
         rewrite -leqNgt addnC leq_add2r => H H1.
@@ -751,10 +710,10 @@ Proof.
     - by rewrite map_ctxinsert -!map_comp.
 Qed.
 
-Theorem subject_reduction :
-  forall ctx t t' ty, t ->r1 t' -> typing ctx t ty -> typing ctx t' ty.
+Theorem subject_reduction ctx t t' ty :
+  t ->r1 t' -> typing ctx t ty -> typing ctx t' ty.
 Proof.
-  move => ctx t t' ty H; move: t t' H ctx ty.
+  move => H; move: t t' H ctx ty.
   refine (reduction1_ind _ _ _ _ _ _ _ _) => /=.
   - move => ty' t1 t2 ctx ty H.
     inversion H; subst; inversion H3; subst => {H H3}.
@@ -764,12 +723,9 @@ Proof.
   - move => t ty' ctx ty H.
     inversion H; subst => {H}; inversion H4; subst => {H4}.
     move: {H2} (substtyp_preserves_typing 0 [:: ty'] H2).
-    rewrite -map_comp /funcomp.
-    set ctx' := map _ _.
-    have -> //: ctx = ctx'.
-      rewrite {}/ctx'.
-      elim: ctx {t ty1} => //= [[ty |]] ctx {1}-> //=.
-      by rewrite subst_shift_cancel_ty //= subnn shift_zero_ty.
+    apply ssr_congr_arrow; f_equal; first by move ->.
+    elim: ctx {t ty1} => //= [[ty |]] ctx {1}-> //=.
+    by rewrite subst_shift_cancel_ty //= subnn shift_zero_ty.
   - move => t1 t1' t2 H IH ctx ty H0; inversion H0; subst; eauto.
   - move => t1 t2 t2' H IH ctx ty H0; inversion H0; subst; eauto.
   - move => ty' t t' H IH ctx ty H0; inversion H0; subst; eauto.
@@ -778,3 +734,13 @@ Proof.
 Qed.
 
 End subject_reduction_proof.
+
+Module strong_normalization_proof.
+
+Import subject_reduction_proof.
+
+Notation SNorm t := (Acc (fun x y => reduction1 y x) t).
+
+
+
+End strong_normalization_proof.
