coq/LC/Debruijn/Untyped.v
@@ -10,6 +10,37 @@ Inductive term : Set := var of nat | app of term & term | abs of term.
 
 Coercion var : nat >-> term.
 
+Fixpoint shift d c t : term :=
+  match t with
+    | var n => var (if c <= n then n + d else n)
+    | app t1 t2 => app (shift d c t1) (shift d c t2)
+    | abs t1 => abs (shift d c.+1 t1)
+  end.
+
+Definition substitutev ts m n : term :=
+  shift n 0 (nth (var (m - n - size ts)) ts (m - n)).
+
+Fixpoint substitute n ts t : term :=
+  match t with
+    | var m => if n <= m then substitutev ts m n else m
+    | app t1 t2 => app (substitute n ts t1) (substitute n ts t2)
+    | abs t' => abs (substitute n.+1 ts t')
+  end.
+
+Reserved Notation "t ->b1 t'" (at level 70, no associativity).
+
+Inductive betared1 : relation term :=
+  | betared1beta t1 t2     : app (abs t1) t2 ->b1 substitute 0 [:: t2] t1
+  | betared1appl t1 t1' t2 : t1 ->b1 t1' -> app t1 t2 ->b1 app t1' t2
+  | betared1appr t1 t2 t2' : t2 ->b1 t2' -> app t1 t2 ->b1 app t1 t2'
+  | betared1abs t t'       : t ->b1 t' -> abs t ->b1 abs t'
+  where "t ->b1 t'" := (betared1 t t').
+
+Notation betared := [* betared1].
+Infix "->b" := betared (at level 70, no associativity).
+
+Hint Resolve betared1beta betared1appl betared1appr betared1abs.
+
 Module Lambda_tactics.
 
 Ltac elimif :=
@@ -34,131 +65,106 @@ End Lambda_tactics.
 
 Import Lambda_tactics.
 
-Fixpoint shift d c t : term :=
-  match t with
-    | var n => var (if c <= n then n + d else n)
-    | app t1 t2 => app (shift d c t1) (shift d c t2)
-    | abs t1 => abs (shift d c.+1 t1)
-  end.
-
-Definition substitutev ts m n : term :=
-  shift n 0 (nth (var (m - n - size ts)) ts (m - n)).
-
-Fixpoint substitute n ts t : term :=
-  match t with
-    | var m => if n <= m then substitutev ts m n else m
-    | app t1 t2 => app (substitute n ts t1) (substitute n ts t2)
-    | abs t' => abs (substitute n.+1 ts t')
-  end.
-
-Lemma shiftzero : forall n t, shift 0 n t = t.
+Lemma shiftzero n t : shift 0 n t = t.
 Proof.
-  move => n t; elim: t n => /=; try congruence.
+  elim: t n => /=; try congruence.
   by move => m n; rewrite addn0 if_same.
 Qed.
 
-Lemma shift_add :
-  forall d d' c c' t, c <= c' <= d + c ->
-  shift d' c' (shift d c t) = shift (d' + d) c t.
+Lemma shift_add d d' c c' t :
+  c <= c' <= d + c -> shift d' c' (shift d c t) = shift (d' + d) c t.
 Proof.
-  move => d d' c c' t; case/andP; elimleq; rewrite leq_add2r; elimleq.
+  case/andP; elimleq; rewrite leq_add2r; elimleq.
   elim: t c d => /=; try (move: addnS; congruence); move => *; elimif_omega.
 Qed.
 
-Lemma shift_shift_distr :
-  forall d c d' c' t,
+Lemma shift_shift_distr d c d' c' t :
   c' <= c -> shift d' c' (shift d c t) = shift d (d' + c) (shift d' c' t).
 Proof.
-  move => d c d' c' t; elimleq; elim: t c' c => /=;
-    try (move: addnS; congruence); move => *; elimif_omega.
+  elimleq; elim: t c' c => /=; try (move: addnS; congruence);
+    move => *; elimif_omega.
 Qed.
 
-Lemma shift_subst_distr :
-  forall n d c ts t, c <= n ->
-  shift d c (substitute n ts t) = substitute (d + n) ts (shift d c t).
+Lemma shift_subst_distr n d c ts t :
+  c <= n -> shift d c (substitute n ts t) = substitute (d + n) ts (shift d c t).
 Proof.
-  move => n d c ts t; elimleq; elim: t c n => /=;
-    try (move: addnS; congruence); move => v c n; elimif_omega.
+  elimleq; elim: t c n => /=; try (move: addnS; congruence);
+    move => v c n; elimif_omega.
   by rewrite /substitutev shift_add ?addn0 ?leq_addl // !subnDA addnK.
 Qed.
 
-Lemma subst_shift_distr :
-  forall n d c ts t,
-  shift d (n + c) (substitute n ts t) =
-  substitute n (map (shift d c) ts) (shift d (size ts + n + c) t).
+Lemma subst_shift_distr n d c ts t :
+  n <= c ->
+  shift d c (substitute n ts t) =
+  substitute n (map (shift d (c - n)) ts) (shift d (size ts + c) t).
 Proof.
-  move => n d c ts t; elim: t n => /=; try (move: addnS addSn; congruence).
+  elimleq; elim: t n => /=; try (move: addnS addSn; congruence).
   move => v n; elimif_omega; rewrite /substitutev.
   - rewrite !nth_default ?size_map /= ?(subnAC _ n) ?subnK; elimif_omega.
-  - rewrite -shift_shift_distr // nth_map' /=.
+  - rewrite addnC -shift_shift_distr // nth_map' /=.
     f_equal; apply nth_equal; rewrite size_map; elimif_omega.
 Qed.
 
-Lemma subst_shift_cancel :
-  forall n d c ts t, c <= n -> size ts + n <= d + c ->
+Lemma subst_shift_cancel n d c ts t :
+  c <= n -> size ts + n <= d + c ->
   substitute n ts (shift d c t) = shift (d - size ts) c t.
 Proof.
-  move => n d c ts t; elimleq; rewrite addnA leq_add2r; elimleq.
-  elim: t c d => /=; try (move: addnS; congruence); move => v c d; elimif_omega.
+  elimleq; rewrite addnA leq_add2r; elimleq; elim: t c d => /=;
+    try (move: addnS; congruence); move => v c d; elimif_omega.
   rewrite /substitutev nth_default /=; elimif_omega.
 Qed.
 
-Lemma subst_subst_distr :
-  forall n m xs ys t,
-  substitute (m + n) xs (substitute m ys t) =
-  substitute m (map (substitute n xs) ys) (substitute (size ys + m + n) xs t).
+Lemma subst_subst_distr n m xs ys t :
+  m <= n ->
+  substitute n xs (substitute m ys t) =
+  substitute m (map (substitute (n - m) xs) ys) (substitute (size ys + n) xs t).
 Proof.
-  move => n m xs ys t; elim: t m => /=; try (move: addnS addSn; congruence).
-  move => v m; elimif_omega; rewrite /substitutev.
+  elimleq; elim: t m => /=; try (move: addnS addSn; congruence);
+    move => v m; elimif_omega; rewrite /substitutev.
   - rewrite (subst_shift_cancel m) // ?size_map; try ssromega.
     rewrite nth_default /= /substitutev; elimif_omega.
-    by rewrite !(nth_map' (shift _ _)) /= subnDA addnK
-      (addnC _ m) addnAC addnK !subnDA (subnAC _ n (size ys)).
-  - rewrite size_map -shift_subst_distr // nth_map' /=.
+    by rewrite !subnDA (subnAC _ n) addKn addnK 2!(subnAC _ m).
+  - rewrite size_map addnC -shift_subst_distr // nth_map' /=.
     f_equal; apply nth_equal; rewrite size_map; elimif_omega.
 Qed.
 
-Lemma subst_app :
-  forall n xs ys t,
+Lemma subst_app n xs ys t :
   substitute n xs (substitute (size xs + n) ys t) = substitute n (xs ++ ys) t.
 Proof.
-  move => n xs ys t; elim: t n => /=; try (move: addnS; congruence).
-  move => v n; rewrite /substitutev nth_cat size_cat; elimif_omega.
+  elim: t n => /=; try (move: addnS; congruence);
+    move => v n; rewrite /substitutev nth_cat size_cat; elimif_omega.
   - by rewrite subst_shift_cancel ?addn0 // addKn addnC !subnDA.
   - rewrite /substitutev; f_equal; apply nth_equal; ssromega.
 Qed.
 
-Lemma subst_nil : forall n t, substitute n [::] t = t.
+Lemma subst_nil n t : substitute n [::] t = t.
 Proof.
-  move => n t; elim: t n => /=; try congruence.
-  move => m n; rewrite /substitutev nth_nil /=; elimif_omega.
+  elim: t n => /=; try congruence; move => m n;
+    rewrite /substitutev nth_nil /=; elimif_omega.
 Qed.
 
-Reserved Notation "t ->b1 t'" (at level 70, no associativity).
+Lemma subst_betared1 n ts t t' :
+  t ->b1 t' -> substitute n ts t ->b1 substitute n ts t'.
+Proof.
+  move => H; move: t t' H n.
+  refine (betared1_ind _ _ _ _ _) => /=; auto => t t' n.
+  by rewrite subst_subst_distr //= add1n subn0.
+Qed.
+
+Module confluence_proof.
+
 Reserved Notation "t ->bp t'" (at level 70, no associativity).
 
-Inductive betared1 : relation term :=
-  | betared1beta : forall t1 t2, app (abs t1) t2 ->b1 substitute 0 [:: t2] t1
-  | betared1appl : forall t1 t1' t2, t1 ->b1 t1' -> app t1 t2 ->b1 app t1' t2
-  | betared1appr : forall t1 t2 t2', t2 ->b1 t2' -> app t1 t2 ->b1 app t1 t2'
-  | betared1abs  : forall t t', t ->b1 t' -> abs t ->b1 abs t'
-  where "t ->b1 t'" := (betared1 t t').
-
 Inductive parred : relation term :=
-  | parredvar  : forall n, var n ->bp var n
-  | parredapp  : forall t1 t1' t2 t2',
-                 t1 ->bp t1' -> t2 ->bp t2' -> app t1 t2 ->bp app t1' t2'
-  | parredabs  : forall t t', t ->bp t' -> abs t ->bp abs t'
-  | parredbeta : forall t1 t1' t2 t2',
-                 t1 ->bp t1' -> t2 ->bp t2' ->
-                 app (abs t1) t2 ->bp substitute 0 [:: t2'] t1'
+  | parredvar n : var n ->bp var n
+  | parredapp t1 t1' t2 t2' :
+    t1 ->bp t1' -> t2 ->bp t2' -> app t1 t2 ->bp app t1' t2'
+  | parredabs t t' : t ->bp t' -> abs t ->bp abs t'
+  | parredbeta t1 t1' t2 t2' :
+    t1 ->bp t1' -> t2 ->bp t2' -> app (abs t1) t2 ->bp substitute 0 [:: t2'] t1'
   where "t ->bp t'" := (parred t t').
 
-Notation betared := [* betared1].
-Infix "->b" := betared (at level 70, no associativity).
-
-Hint Resolve betared1beta betared1appl betared1appr betared1abs
-    parredvar parredapp parredabs parredbeta.
+Hint Resolve parredvar parredapp parredabs parredbeta.
 
 Function reduce_all_redex t : term :=
   match t with
@@ -169,26 +175,26 @@ Function reduce_all_redex t : term :=
     | abs t' => abs (reduce_all_redex t')
   end.
 
-Lemma parred_refl : forall t, parred t t.
+Lemma parred_refl t : parred t t.
 Proof.
-  elim; auto.
+  elim: t; auto.
 Qed.
 
-Lemma betaredappl : forall t1 t1' t2, t1 ->b t1' -> app t1 t2 ->b app t1' t2.
+Lemma betaredappl t1 t1' t2 : t1 ->b t1' -> app t1 t2 ->b app t1' t2.
 Proof.
-  move => t1 t1' t2; elim => // {t1 t1'} t1 t1' t1'' H H0 H1.
+  elim => // {t1 t1'} t1 t1' t1'' H H0 H1.
   apply rt1n_trans with (app t1' t2) => //; auto.
 Qed.
 
-Lemma betaredappr : forall t1 t2 t2', t2 ->b t2' -> app t1 t2 ->b app t1 t2'.
+Lemma betaredappr t1 t2 t2' : t2 ->b t2' -> app t1 t2 ->b app t1 t2'.
 Proof.
-  move => t1 t2 t2'; elim => // {t2 t2'} t2 t2' t2'' H H0 H1.
+  elim => // {t2 t2'} t2 t2' t2'' H H0 H1.
   apply rt1n_trans with (app t1 t2') => //; auto.
 Qed.
 
-Lemma betaredabs : forall t t', t ->b t' -> abs t ->b abs t'.
+Lemma betaredabs t t' : t ->b t' -> abs t ->b abs t'.
 Proof.
-  move => t t'; elim => // {t t'} t t' t'' H H0 H1.
+  elim => // {t t'} t t' t'' H H0 H1.
   apply rt1n_trans with (abs t') => //; auto.
 Qed.
 
@@ -210,39 +216,30 @@ Proof.
     by apply rtc_step.
 Qed.
 
-Lemma subst_betared1 :
-  forall n ts t t', t ->b1 t' -> substitute n ts t ->b1 substitute n ts t'.
+Lemma shift_parred t t' d c : t ->bp t' -> shift d c t ->bp shift d c t'.
 Proof.
-  move => n t1 t2 t2' H; move: t2 t2' H n.
-  refine (betared1_ind _ _ _ _ _) => /=; auto => t2 t2' n.
-  by rewrite (subst_subst_distr n 0) /= !add1n.
-Qed.
-
-Lemma shift_parred :
-  forall t t' d c, t ->bp t' -> shift d c t ->bp shift d c t'.
-Proof.
-  move => t t' d c H; move: t t' H d c.
+  move => H; move: t t' H d c.
   refine (parred_ind _ _ _ _ _) => //=; auto => t1 t1' t2 t2' H H0 H1 H2 d c.
-  rewrite (subst_shift_distr 0) /= !add1n; auto.
+  rewrite subst_shift_distr //= add1n subn0; auto.
 Qed.
 
-Lemma subst_parred :
-  forall n ps t t', Forall (prod_curry parred) ps -> t ->bp t' ->
+Lemma subst_parred n ps t t' :
+  Forall (prod_curry parred) ps -> t ->bp t' ->
   substitute n [seq fst p | p <- ps] t ->bp
   substitute n [seq snd p | p <- ps] t'.
 Proof.
-  move => n ps t t' H H0; move: t t' H0 n.
+  move => H H0; move: t t' H0 n.
   refine (parred_ind _ _ _ _ _) => /=; auto.
   - move => v n; elimif; rewrite /substitutev !size_map; apply shift_parred.
     elim: {v n H0} ps (v - n) H => //= [[t t']] ps IH [| v] [] //= H H0.
     by rewrite subSS; apply IH.
   - move => t1 t1' t2 t2' H0 H1 H2 H3 n.
-    by rewrite (subst_subst_distr n 0) /= !add1n; auto.
+    by rewrite subst_subst_distr //= add1n subn0; auto.
 Qed.
 
-Lemma parred_all_lemma : forall t t', t ->bp t' -> t' ->bp reduce_all_redex t.
+Lemma parred_all_lemma t t' : t ->bp t' -> t' ->bp reduce_all_redex t.
 Proof with auto.
-  move => t; elim/reduce_all_redex_ind: {t}_.
+  elim/reduce_all_redex_ind: {t}_ t'.
   - by move => t n H t' H0; inversion H0; subst.
   - move => _ t1 t2 _ H H0 t' H1; inversion H1; subst.
     - inversion H4; subst...
@@ -262,3 +259,5 @@ Proof.
   apply (rtc_confluent' parred
     betared1_in_parred parred_in_betared parred_confluent).
 Qed.
+
+End confluence_proof.
