coq/lib/Relations_ext.v
@@ -14,41 +14,39 @@ Notation "[ * R ]" :=
 
 Hint Resolve rt1n_refl.
 
-Lemma rtc_trans' : forall A R, transitive A [* R].
+Lemma rtc_trans' A R : transitive A [* R].
 Proof.
-  move => A R t1 t2 t3.
+  move => t1 t2 t3.
   rewrite -!clos_rt_rt1n_iff.
   apply rt_trans.
 Qed.
 
-Lemma rtc_step : forall (A : Set) (R : relation A), inclusion R [* R].
+Lemma rtc_step A (R : relation A) : inclusion R [* R].
 Proof.
-  by move => A R x y H; apply rt1n_trans with y.
+  by move => x y H; apply rt1n_trans with y.
 Qed.
 
-Lemma rtc_map :
-  forall A (R R' : relation A), inclusion R R' -> inclusion [* R] [* R'].
+Lemma rtc_map A (R R' : relation A) : inclusion R R' -> inclusion [* R] [* R'].
 Proof.
-  move => A R R' H.
-  refine (clos_refl_trans_1n_ind A R _ _ _) => // t1 t2 t3 ? ? ?.
+  move => H.
+  refine (clos_refl_trans_1n_ind A R _ _ _) => // t1 t2 t3 H0 H1 H2.
   apply rt1n_trans with t2; auto.
 Qed.
 
-Lemma rtc_nest_elim : forall A (R : relation A), same_relation [* [* R]] [* R].
+Lemma rtc_nest_elim A (R : relation A) : same_relation [* [* R]] [* R].
 Proof.
-  move => A R t1 t2; split.
+  move => t1 t2; split.
   - move: t1 t2; refine (clos_refl_trans_1n_ind A _ _ _ _) => //.
     by move => t1 t2 t3 H _ H0; apply rtc_trans' with t2.
   - apply clos_rt1n_step.
 Qed.
 
-Lemma rtc_semi_confluent :
-  forall A (R R' : relation A),
+Lemma rtc_semi_confluent A (R R' : relation A) :
   (forall t1 t2 t3, R t1 t2 -> R' t1 t3 -> exists t4, R' t2 t4 /\ R t3 t4) ->
   (forall t1 t2 t3, [* R] t1 t2 -> R' t1 t3 ->
     exists t4, R' t2 t4 /\ [* R] t3 t4).
 Proof.
-  move => A R R' H t1 t2 t3 H0; move: t1 t2 H0 t3.
+  move => H t1 t2 t3 H0; move: t1 t2 H0 t3.
   refine (clos_refl_trans_1n_ind A R _ _ _).
   - by move => t1 t3 H0; exists t3.
   - move => t1 t1' t2 H0 H1 IH t3 H2.
@@ -57,29 +55,27 @@ Proof.
     by apply rt1n_trans with t3'.
 Qed.
 
-Lemma rtc_confluent :
-  forall A (R : relation A), confluent R -> confluent [* R].
+Lemma rtc_confluent A (R : relation A) : confluent R -> confluent [* R].
 Proof.
-  move => A R H.
+  move => H.
   apply rtc_semi_confluent.
   move: (rtc_semi_confluent R H) => {H} H t1 t2 t3 H0 H1.
   by case: (H t1 t3 t2 H1 H0) => t4; case => H2 H3; exists t4.
 Qed.
 
-Lemma rtc_confluent' : forall A (R R' : relation A),
+Lemma rtc_confluent' A (R R' : relation A) :
   inclusion R R' -> inclusion R' [* R] -> confluent R' -> confluent [* R].
 Proof.
-  move => A R R' H H0 H1 t1 t2 t3 H2 H3.
+  move => H H0 H1 t1 t2 t3 H2 H3.
   case (rtc_confluent H1 (rtc_map _ H H2) (rtc_map _ H H3))
-    => t4 [? ?].
+    => t4 [H4 H5].
   by exists t4; split; rewrite -rtc_nest_elim; apply (rtc_map _ H0).
 Qed.
 
-Theorem rtc_preservation :
-  forall A (P : A -> Prop) (R : relation A),
+Theorem rtc_preservation A (P : A -> Prop) (R : relation A) :
   (forall x y, R x y -> P x -> P y) -> forall x y, [* R] x y -> P x -> P y.
 Proof.
-  move => A P R H.
+  move => H.
   refine (clos_refl_trans_1n_ind A R _ _ _) => //= x y z H0 _ H1 H2.
   exact (H1 (H x y H0 H2)).
 Qed.
