coq/lib/seq_ext.v
@@ -10,114 +10,99 @@ Variable (A B : Type).
 
 (* drop and take *)
 
-Theorem drop_addn :
-  forall n m (xs : seq A), drop n (drop m xs) = drop (n + m) xs.
+Theorem drop_addn n m (xs : seq A) : drop n (drop m xs) = drop (n + m) xs.
 Proof.
-  move => n; elim => [| m IH] [] // x xs.
+  elim: m xs => [| m IH] [] // x xs.
   - by rewrite addn0.
   - by rewrite addnS /= IH.
 Qed.
 
-Theorem take_minn :
-  forall n m (xs : seq A), take n (take m xs) = take (minn n m) xs.
+Theorem take_minn n m (xs : seq A) : take n (take m xs) = take (minn n m) xs.
 Proof.
-  by elim => [| n IH] [| m] [] // x xs; rewrite minnSS /= IH.
+  by elim: n m xs => [| n IH] [| m] [] // x xs; rewrite minnSS /= IH.
 Qed.
 
-Theorem drop_take_distr :
-  forall n m (xs : seq A), drop n (take m xs) = take (m - n) (drop n xs).
+Theorem drop_take_distr n m (xs : seq A) :
+  drop n (take m xs) = take (m - n) (drop n xs).
 Proof.
-  elim => [m xs | n IH [xs | m [] //= _ xs]].
+  elim: n m xs => [m xs | n IH [xs | m [] //= _ xs]].
   - by rewrite !drop0 subn0.
   - by rewrite sub0n !take0.
   - by rewrite subSS IH.
 Qed.
 
-Theorem take_drop_distr :
-  forall n m (xs : seq A), take n (drop m xs) = drop m (take (n + m) xs).
+Theorem take_drop_distr n m (xs : seq A) :
+  take n (drop m xs) = drop m (take (n + m) xs).
 Proof.
-  by move => n m xs; rewrite drop_take_distr addnK.
+  by rewrite drop_take_distr addnK.
 Qed.
 
-Theorem drop_take_nil : forall n (xs : seq A), drop n (take n xs) = [::].
+Theorem drop_take_nil n (xs : seq A) : drop n (take n xs) = [::].
 Proof.
-  by move => n xs; rewrite drop_take_distr subnn take0.
+  by rewrite drop_take_distr subnn take0.
 Qed.
 
-Theorem size_take : forall n (xs : seq A), size (take n xs) = minn n (size xs).
+Theorem size_take n (xs : seq A) : size (take n xs) = minn n (size xs).
 Proof.
-  elim => [xs | n IH [] //= _ xs].
+  elim: n xs => [xs | n IH [] //= _ xs].
   - by rewrite take0 min0n.
   - by rewrite minnSS IH.
 Qed.
 
 (* nth *)
 
-Theorem nth_map' :
-  forall (f : A -> B) x xs n, f (nth x xs n) = nth (f x) (map f xs) n.
+Theorem nth_map' (f : A -> B) x xs n : f (nth x xs n) = nth (f x) (map f xs) n.
 Proof.
-  move => f x; elim => /=.
-  - by move => n; rewrite !nth_nil.
-  - by move => x' xs IH [].
+  by elim: xs n => [n | x' xs IH []] //=; rewrite !nth_nil.
 Qed.
 
-Theorem nth_equal :
-  forall (a b : A) xs n, (size xs <= n -> a = b) -> nth a xs n = nth b xs n.
+Theorem nth_equal (a b : A) xs n :
+  (size xs <= n -> a = b) -> nth a xs n = nth b xs n.
 Proof.
-  move => a b; elim.
-  by move => n /= ->.
-  by move => x xs IH [].
+  by elim: xs n => [n /= -> | x xs IH []].
 Qed.
 
 End Seq.
 
 (* context *)
 
-Notation ctxindex xs n x := (Some x = nth None xs n).
-Notation ctxleq xs ys := (forall n a, ctxindex xs n a -> ctxindex ys n a).
-Infix "<=c" := ctxleq (at level 70, no associativity).
-
 Definition context A := (seq (option A)).
 
 Definition ctxinsert A xs ys n : context A :=
   take n ys ++ nseq (n - size ys) None ++ xs ++ drop n ys.
 
+Notation ctxindex xs n x := (Some x = nth None xs n).
+Notation ctxleq xs ys := (forall n a, ctxindex xs n a -> ctxindex ys n a).
+Infix "<=c" := ctxleq (at level 70, no associativity).
+Notation ctxmap f xs := (map (omap f) xs).
+
 Section Context.
 
 Variable (A B : Type).
 
-Theorem ctxindex_map :
-  forall (f : A -> B) xs n x,
-  ctxindex xs n x -> ctxindex (map (omap f) xs) n (f x).
+Theorem ctxindex_map (f : A -> B) xs n x :
+  ctxindex xs n x -> ctxindex (ctxmap f xs) n (f x).
 Proof.
-  by move => f; elim => [| x xs IH] [] //= x' <-.
+  by elim: xs n x => [| x xs IH] [] //= x' <-.
 Qed.
 
-Theorem size_ctxinsert :
-  forall (xs ys : context A) n,
+Theorem size_ctxinsert (xs ys : context A) n :
   size (ctxinsert xs ys n) = size xs + maxn n (size ys).
 Proof.
-  move => xs ys n.
-  rewrite /ctxinsert !size_cat size_nseq size_take size_drop.
-  ssromega.
+  rewrite /ctxinsert !size_cat size_nseq size_take size_drop; ssromega.
 Qed.
 
-Theorem map_ctxinsert :
-  forall (f : A -> B) xs ys n,
-  map (omap f) (ctxinsert xs ys n) =
-  ctxinsert (map (omap f) xs) (map (omap f) ys) n.
+Theorem map_ctxinsert (f : A -> B) xs ys n :
+  ctxmap f (ctxinsert xs ys n) = ctxinsert (ctxmap f xs) (ctxmap f ys) n.
 Proof.
-  move => f xs ys n.
   by rewrite /ctxinsert !map_cat map_take map_nseq size_map map_drop.
 Qed.
 
-Theorem nth_ctxinsert :
-  forall (xs ys : context A) n m,
+Theorem nth_ctxinsert (xs ys : context A) n m :
   nth None (ctxinsert xs ys n) m =
   if m < n then nth None ys m else
   if m < n + size xs then nth None xs (m - n) else nth None ys (m - size xs).
 Proof.
-  move => xs ys n m.
   rewrite /ctxinsert !nth_cat size_take size_nseq -subnDA.
   replace (minn n (size ys) + (n - size ys)) with n by ssromega.
   do! case: ifP; try ssromega.
@@ -127,49 +112,48 @@ Proof.
   - move => H _ _ _ _; rewrite nth_drop; f_equal; ssromega.
 Qed.
 
-Theorem ctxleq_refl : forall (xs : context A), ctxleq xs xs.
+Theorem ctxleq_refl (xs : context A) : ctxleq xs xs.
 Proof.
   done.
 Qed.
 
-Theorem ctxleq_trans :
-  forall (xs ys zs : context A), ctxleq xs ys -> ctxleq ys zs -> ctxleq xs zs.
+Theorem ctxleq_trans (xs ys zs : context A) :
+  ctxleq xs ys -> ctxleq ys zs -> ctxleq xs zs.
 Proof.
   auto.
 Qed.
 
-Theorem ctxleq_nil : forall (xs : context A), ctxleq [::] xs.
+Theorem ctxleq_nil (xs : context A) : ctxleq [::] xs.
 Proof.
-  by move => xs n a; rewrite nth_nil.
+  by move => n a; rewrite nth_nil.
 Qed.
 
-Theorem ctxleq_appl :
-  forall (xs ys zs : context A), ctxleq ys zs -> ctxleq (xs ++ ys) (xs ++ zs).
+Theorem ctxleq_appl (xs ys zs : context A) :
+  ctxleq ys zs -> ctxleq (xs ++ ys) (xs ++ zs).
 Proof.
-  by elim => // x xs IH ys zs H [] //=; apply IH.
+  by elim: xs ys zs => // x xs IH ys zs H [] //=; apply IH.
 Qed.
 
-Theorem ctxleq_appr : forall (xs ys : context A), ctxleq xs (xs ++ ys).
+Theorem ctxleq_appr (xs ys : context A) : ctxleq xs (xs ++ ys).
 Proof.
-  by move => xs ys; elim: xs => [n a | x xs H []] //=; rewrite nth_nil.
+  by elim: xs => [n a | x xs H []] //=; rewrite nth_nil.
 Qed.
 
-Theorem ctxleq_app :
-  forall (xs xs' ys ys' : context A), size xs = size xs' ->
-  ctxleq xs xs' -> ctxleq ys ys' -> ctxleq (xs ++ ys) (xs' ++ ys').
+Theorem ctxleq_app (xs xs' ys ys' : context A) :
+  size xs = size xs' -> ctxleq xs xs' -> ctxleq ys ys' ->
+  ctxleq (xs ++ ys) (xs' ++ ys').
 Proof.
-  elim => [| x xs IH] [] //= x' xs' ys ys' [H] H0 H1 [| n] a /=.
+  elim: xs xs' ys ys' => [| x xs IH] [] //= x' xs' ys ys' [H] H0 H1 [| n] a /=.
   - apply (H0 0 a).
   - apply IH => // m; apply (H0 m.+1).
 Qed.
 
 End Context.
 
-Theorem ctxleq_map :
-  forall A B (f : A -> B) xs ys,
-  ctxleq xs ys -> ctxleq (map (omap f) xs) (map (omap f) ys).
+Theorem ctxleq_map A B (f : A -> B) xs ys :
+  ctxleq xs ys -> ctxleq (ctxmap f xs) (ctxmap f ys).
 Proof.
-  move => A B f xs ys H n y; move: {H} (H n).
+  move => H n y; move: {H} (H n).
   rewrite -!(nth_map' (omap f) None).
   by case: (nth None xs n) => // a H; rewrite -(H a).
 Qed.
@@ -186,18 +170,16 @@ Proof.
   move => A P Q xs H; elim: xs; firstorder.
 Qed.
 
-Theorem Forall_map :
-  forall (A B : Type) (f : A -> B) (P : B -> Prop) xs,
+Theorem Forall_map (A B : Type) (f : A -> B) P xs :
   Forall P (map f xs) <-> Forall (P \o f) xs.
 Proof.
-  by move => A B f P; elim => //= x xs ->.
+  by elim: xs => //= x xs ->.
 Qed.
 
-Theorem Forall_nth :
-  forall (A : Type) (P : A -> Prop) x xs m,
+Theorem Forall_nth (A : Type) (P : A -> Prop) x xs m :
   m < size xs -> Forall P xs -> P (nth x xs m).
 Proof.
-  move => A P x0; elim => // x xs IH [].
+  elim: xs m => // x' xs IH [].
   - by move => _ /= [].
   - by move => n; rewrite /= ltnS => H [_]; apply IH.
 Qed.
